Test/civl/large-samples/shared-vector.bpl
@@ -4,7 +4,7 @@
 ////////////////////////////////////////////////////////////////////////////////
 // Shared integer array implementation
 
-var {:layer 2, 3} IntArrayPool: Map (Loc IntArray) (Vec int);
+var {:layer 2, 3} IntArrayPool: Map (One (Loc IntArray)) (Vec int);
 
 datatype IntArray {
   IntArray(
@@ -13,15 +13,15 @@ datatype IntArray {
   )
 }
 
-var {:layer 0, 2} {:linear} IntArrayPoolLow: Map (Loc IntArray) IntArray;
+var {:layer 0, 2} {:linear} IntArrayPoolLow: Map (One (Loc IntArray)) IntArray;
 
 yield invariant {:layer 2} IntArrayDom();
 preserves IntArrayPool->dom == IntArrayPoolLow->dom;
 
 yield invariant {:layer 2} Yield(loc_iv: Loc IntArray);
-preserves Map_Contains(IntArrayPoolLow, loc_iv);
+preserves Map_Contains(IntArrayPoolLow, One(loc_iv));
 preserves
-  (var intvec_low, intvec_high := Map_At(IntArrayPoolLow, loc_iv), Map_At(IntArrayPool, loc_iv);
+  (var intvec_low, intvec_high := Map_At(IntArrayPoolLow, One(loc_iv)), Map_At(IntArrayPool, One(loc_iv));
     intvec_low->mutexes->dom == intvec_low->values->dom &&
     intvec_low->mutexes->dom->val == (lambda i: int :: 0 <= i && i < Vec_Len(intvec_high)) &&
     (forall j: int:: 0 <= j && j < Vec_Len(intvec_high) ==> Map_Contains(MutexPool, Map_At(intvec_low->mutexes, j)->val)) &&
@@ -33,8 +33,8 @@ modifies IntArrayPool;
   var {:linear} one_loc_iv: One (Loc IntArray);
   call one_loc_iv := Loc_New();
   loc_iv := one_loc_iv->val;
-  assume !Map_Contains(IntArrayPool, loc_iv);
-  IntArrayPool := Map_Update(IntArrayPool, loc_iv, v);
+  assume !Map_Contains(IntArrayPool, One(loc_iv));
+  IntArrayPool := Map_Update(IntArrayPool, One(loc_iv), v);
 }
 yield procedure {:layer 2} IntArray_Alloc(v: Vec int) returns (loc_iv: Loc IntArray)
 refines Atomic_IntArray_Alloc;
@@ -76,14 +76,14 @@ preserves call IntArrayDom();
   call one_loc_iv := Loc_New();
   loc_iv := one_loc_iv->val;
   call AddIntArrayToPool(one_loc_iv, intvec);
-  call {:layer 2} IntArrayPool := Copy(Map_Update(IntArrayPool, one_loc_iv->val, v));
+  call {:layer 2} IntArrayPool := Copy(Map_Update(IntArrayPool, one_loc_iv, v));
 }
 
 atomic action {:layer 3} Atomic_IntArray_Read({:linear} tid: One Tid, loc_iv: Loc IntArray, i: int) returns (v: int)
 {
   var vec: Vec int;
-  assert Map_Contains(IntArrayPool, loc_iv);
-  vec := Map_At(IntArrayPool, loc_iv);
+  assert Map_Contains(IntArrayPool, One(loc_iv));
+  vec := Map_At(IntArrayPool, One(loc_iv));
   assert Vec_Contains(vec, i);
   v := Vec_Nth(vec, i);
 }
@@ -109,11 +109,11 @@ atomic action {:layer 3} Atomic_IntArray_Write({:linear} tid: One Tid, loc_iv: L
 modifies IntArrayPool;
 {
   var vec: Vec int;
-  assert Map_Contains(IntArrayPool, loc_iv);
-  vec := Map_At(IntArrayPool, loc_iv);
+  assert Map_Contains(IntArrayPool, One(loc_iv));
+  vec := Map_At(IntArrayPool, One(loc_iv));
   assert Vec_Contains(vec, i);
   vec := Vec_Update(vec, i, v);
-  IntArrayPool := Map_Update(IntArrayPool, loc_iv, vec);
+  IntArrayPool := Map_Update(IntArrayPool, One(loc_iv), vec);
 }
 yield procedure {:layer 2} IntArray_Write({:linear} tid: One Tid, loc_iv: Loc IntArray, i: int, v: int)
 refines Atomic_IntArray_Write;
@@ -132,18 +132,18 @@ preserves call Yield(loc_iv);
   cell_int := Cell(one_loc_int, v);
   call Locked_PutOwnedLocInt(tid, loc_iv, i, cell_int);
   call Mutex_Release(tid, loc_mutex);
-  call {:layer 2} IntArrayPool := Copy(Map_Update(IntArrayPool, loc_iv, Vec_Update(Map_At(IntArrayPool, loc_iv), i, v)));
+  call {:layer 2} IntArrayPool := Copy(Map_Update(IntArrayPool, One(loc_iv), Vec_Update(Map_At(IntArrayPool, One(loc_iv)), i, v)));
 }
 
 atomic action {:layer 3} Atomic_IntArray_Swap({:linear} tid: One Tid, loc_iv: Loc IntArray, i: int, j: int)
 modifies IntArrayPool;
 {
   var vec: Vec int;
-  assert Map_Contains(IntArrayPool, loc_iv);
-  vec := Map_At(IntArrayPool, loc_iv);
+  assert Map_Contains(IntArrayPool, One(loc_iv));
+  vec := Map_At(IntArrayPool, One(loc_iv));
   assert Vec_Contains(vec, i) && Vec_Contains(vec, j);
   vec := Vec_Swap(vec, i, j);
-  IntArrayPool := Map_Update(IntArrayPool, loc_iv, vec);
+  IntArrayPool := Map_Update(IntArrayPool, One(loc_iv), vec);
 }
 yield procedure {:layer 2} IntArray_Swap({:linear} tid: One Tid, loc_iv: Loc IntArray, i: int, j: int)
 refines Atomic_IntArray_Swap;
@@ -157,8 +157,8 @@ preserves call Yield(loc_iv);
     return;
   }
 
-  assert {:layer 2} Map_Contains(IntArrayPool, loc_iv);
-  assert {:layer 2} (var vec := Map_At(IntArrayPool, loc_iv); Vec_Contains(vec, i) && Vec_Contains(vec, j));
+  assert {:layer 2} Map_Contains(IntArrayPool, One(loc_iv));
+  assert {:layer 2} (var vec := Map_At(IntArrayPool, One(loc_iv)); Vec_Contains(vec, i) && Vec_Contains(vec, j));
 
   // deadlock avoidance
   if (i < j) {
@@ -168,23 +168,23 @@ preserves call Yield(loc_iv);
   }
 
   call IntArray_Swap_Helper(tid, loc_iv, i', j');
-  call {:layer 2} IntArrayPool := Copy(Map_Update(IntArrayPool, loc_iv, Vec_Swap(Map_At(IntArrayPool, loc_iv), i', j')));
+  call {:layer 2} IntArrayPool := Copy(Map_Update(IntArrayPool, One(loc_iv), Vec_Swap(Map_At(IntArrayPool, One(loc_iv)), i', j')));
 }
 
 yield atomic procedure {:layer 2} IntArray_Swap_Helper({:linear} tid: One Tid, loc_iv: Loc IntArray, i: int, j: int)
 requires {:layer 2} i < j;
-requires {:layer 2} Map_Contains(IntArrayPoolLow, loc_iv);
+requires {:layer 2} Map_Contains(IntArrayPoolLow, One(loc_iv));
 requires {:layer 2}
-  (var intArray := Map_At(IntArrayPoolLow, loc_iv);
+  (var intArray := Map_At(IntArrayPoolLow, One(loc_iv));
     (var mutexes, values := intArray->mutexes, intArray->values;
       Map_Contains(mutexes, i) && Map_Contains(mutexes, j) && Map_Contains(values, i) && Map_Contains(values, j) && 
       Map_Contains(MutexPool, Map_At(mutexes, i)->val) && Map_Contains(MutexPool, Map_At(mutexes, j)->val)));
 ensures {:layer 2}
-  (var intArray := Map_At(old(IntArrayPoolLow), loc_iv);
+  (var intArray := Map_At(old(IntArrayPoolLow), One(loc_iv));
     (var values := intArray->values; 
       (var cell_int_i, cell_int_j := Map_At(values, i), Map_At(values, j);
         (var values' := Map_Update(Map_Update(values, i, cell_int_j), j, cell_int_i);
-          IntArrayPoolLow == Map_Update(old(IntArrayPoolLow), loc_iv, IntArray(intArray->mutexes, values'))))));
+          IntArrayPoolLow == Map_Update(old(IntArrayPoolLow), One(loc_iv), IntArray(intArray->mutexes, values'))))));
 ensures {:layer 2} MutexPool == old(MutexPool);
 {
   var loc_mutex_i: Loc int;
@@ -212,7 +212,8 @@ modifies IntArrayPoolLow;
   var {:linear "no_collect_keys"} mutexes: Map int (One (Loc int));
   var {:linear "no_collect_keys"} values: Map int (Cell (Loc int) int);
 
-  call one_loc_iv, intvec := Map_Get(IntArrayPoolLow, loc_iv);
+  one_loc_iv := One(loc_iv);
+  call intvec := Map_GetValue(IntArrayPoolLow, one_loc_iv);
   IntArray(mutexes, values) := intvec;
 
   // the following lines are added over Atomic_GetOwnedLocInt
@@ -221,7 +222,7 @@ modifies IntArrayPoolLow;
 
   call cell_int := Map_GetValue(values, i);
   intvec := IntArray(mutexes, values);
-  call Map_Put(IntArrayPoolLow, one_loc_iv, intvec);
+  call Map_PutValue(IntArrayPoolLow, one_loc_iv, intvec);
 }
 yield procedure {:layer 1} Locked_GetOwnedLocInt({:linear} tid: One Tid, loc_iv: Loc IntArray, i: int) returns ({:linear} cell_int: Cell (Loc int) int)
 refines Atomic_Locked_GetOwnedLocInt;
@@ -237,7 +238,8 @@ modifies IntArrayPoolLow;
   var {:linear "no_collect_keys"} mutexes: Map int (One (Loc int));
   var {:linear "no_collect_keys"} values: Map int (Cell (Loc int) int);
 
-  call one_loc_iv, intvec := Map_Get(IntArrayPoolLow, loc_iv);
+  one_loc_iv := One(loc_iv);
+  call intvec := Map_GetValue(IntArrayPoolLow, one_loc_iv);
   IntArray(mutexes, values) := intvec;
 
   // the following lines are added over Atomic_PutOwnedLocInt
@@ -246,7 +248,7 @@ modifies IntArrayPoolLow;
 
   call Map_PutValue(values, i, cell_int);
   intvec := IntArray(mutexes, values);
-  call Map_Put(IntArrayPoolLow, one_loc_iv, intvec);
+  call Map_PutValue(IntArrayPoolLow, one_loc_iv, intvec);
 }
 yield procedure {:layer 1} Locked_PutOwnedLocInt({:linear} tid: One Tid, loc_iv: Loc IntArray, i: int, {:linear_in} cell_int: Cell (Loc int) int)
 refines Atomic_Locked_PutOwnedLocInt;
@@ -263,13 +265,14 @@ refines right action {:layer 1, 2} _
   var {:linear "no_collect_keys"} values: Map int (Cell (Loc int) int);
   var {:linear} one_loc_mutex: One (Loc int);
 
-  call one_loc_iv, intvec := Map_Get(IntArrayPoolLow, loc_iv);
+  one_loc_iv := One(loc_iv);
+  call intvec := Map_GetValue(IntArrayPoolLow, one_loc_iv);
   IntArray(mutexes, values) := intvec;
   call one_loc_mutex := Map_GetValue(mutexes, i);
   loc_mutex := one_loc_mutex->val;
   call Map_PutValue(mutexes, i, one_loc_mutex);
   intvec := IntArray(mutexes, values);
-  call Map_Put(IntArrayPoolLow, one_loc_iv, intvec);
+  call Map_PutValue(IntArrayPoolLow, one_loc_iv, intvec);
 }
 
 yield procedure {:layer 0} GetOwnedLocInt(loc_iv: Loc IntArray, i: int) returns ({:linear} cell_int: Cell (Loc int) int);
@@ -280,11 +283,12 @@ refines atomic action {:layer 1, 1} _
   var {:linear "no_collect_keys"} mutexes: Map int (One (Loc int));
   var {:linear "no_collect_keys"} values: Map int (Cell (Loc int) int);
 
-  call one_loc_iv, intvec := Map_Get(IntArrayPoolLow, loc_iv);
+  one_loc_iv := One(loc_iv);
+  call intvec := Map_GetValue(IntArrayPoolLow, one_loc_iv);
   IntArray(mutexes, values) := intvec;
   call cell_int := Map_GetValue(values, i);
   intvec := IntArray(mutexes, values);
-  call Map_Put(IntArrayPoolLow, one_loc_iv, intvec);
+  call Map_PutValue(IntArrayPoolLow, one_loc_iv, intvec);
 }
 
 yield procedure {:layer 0} PutOwnedLocInt(loc_iv: Loc IntArray, i: int, {:linear_in} cell_int: Cell (Loc int) int);
@@ -295,17 +299,18 @@ refines atomic action {:layer 1, 1} _
   var {:linear "no_collect_keys"} mutexes: Map int (One (Loc int));
   var {:linear "no_collect_keys"} values: Map int (Cell (Loc int) int);
 
-  call one_loc_iv, intvec := Map_Get(IntArrayPoolLow, loc_iv);
+  one_loc_iv := One(loc_iv);
+  call intvec := Map_GetValue(IntArrayPoolLow, one_loc_iv);
   IntArray(mutexes, values) := intvec;
   call Map_PutValue(values, i, cell_int);
   intvec := IntArray(mutexes, values);
-  call Map_Put(IntArrayPoolLow, one_loc_iv, intvec);
+  call Map_PutValue(IntArrayPoolLow, one_loc_iv, intvec);
 }
 
 yield procedure {:layer 0} AddIntArrayToPool({:linear_in} one_loc_iv: One (Loc IntArray), {:linear_in} intvec: IntArray);
 refines atomic action {:layer 1, 2} _
 {
-  call Map_Put(IntArrayPoolLow, one_loc_iv, intvec);
+  call Map_PutValue(IntArrayPoolLow, one_loc_iv, intvec);
 }
 
 type Tid;
