Test/civl/large-samples/treiber-stack.bpl
@@ -1,16 +1,16 @@
-// RUN: %parallel-boogie -lib:base -lib:node -timeLimit:0 -vcsSplitOnEveryAssert "%s" > "%t"
+// RUN: %parallel-boogie -lib:base -lib:node -timeLimit:0 "%s" > "%t"
 // RUN: %diff "%s.expect" "%t"
 
 type TaggedLocNode V = TaggedLoc (Node V) Unit;
 
-datatype Treiber<V> { Treiber(top: Option (LocNode V), {:linear} nodes: Map (LocNode V) (Node V)) }
+datatype Treiber<V> { Treiber(top: Option (LocNode V), {:linear} nodes: Map (One (LocNode V)) (Node V)) }
 type LocTreiber V = Loc (Treiber V);
 type TaggedLocTreiber V = TaggedLoc (Treiber V) Unit;
 
 type X; // module type parameter
 
-var {:layer 4, 5} TreiberPool: Map (LocTreiber X) (Vec X);
-var {:layer 0, 4} {:linear} TreiberPoolLow: Map (LocTreiber X) (Treiber X);
+var {:layer 4, 5} TreiberPool: Map (One (LocTreiber X)) (Vec X);
+var {:layer 0, 4} {:linear} TreiberPoolLow: Map (One (LocTreiber X)) (Treiber X);
 
 /// Proof outline
 /*
@@ -26,41 +26,46 @@ Layer 4: Introduce TreiberPool and abstract TreiberPoolLow to TreiberPool
 
 /// Yield invariants
 
-function {:inline} Domain(ts: Map (LocTreiber X) (Treiber X), loc_t: LocTreiber X): Set (LocNode X) {
-  ts->val[loc_t]->nodes->dom
+function {:inline} Domain(ts: Map (One (LocTreiber X)) (Treiber X), loc_t: LocTreiber X): Set (One (LocNode X)) {
+  ts->val[One(loc_t)]->nodes->dom
+}
+
+function {:inline} ListInDomain(t: Treiber X): bool {
+  (forall x: LocNode X:: BetweenSet(t->nodes->val, t->top, None())[x] ==> Set_Contains(t->nodes->dom, One(x)))
 }
 
 yield invariant {:layer 1} Yield();
 
 yield invariant {:layer 2} TopInStack(loc_t: LocTreiber X);
-preserves Map_Contains(TreiberPoolLow, loc_t);
-preserves (var loc_n := Map_At(TreiberPoolLow, loc_t)->top; loc_n is None || Set_Contains(Domain(TreiberPoolLow, loc_t), loc_n->t));
-preserves (forall loc_n: LocNode X :: Set_Contains(Domain(TreiberPoolLow, loc_t), loc_n) ==>
-              (var loc_n' := Map_At(Map_At(TreiberPoolLow, loc_t)->nodes, loc_n)->next; loc_n' is None || Set_Contains(Domain(TreiberPoolLow, loc_t), loc_n'->t)));
+preserves Map_Contains(TreiberPoolLow, One(loc_t));
+preserves (var loc_n := Map_At(TreiberPoolLow, One(loc_t))->top; loc_n is None || Set_Contains(Domain(TreiberPoolLow, loc_t), One(loc_n->t)));
+preserves (forall loc_n: LocNode X :: Set_Contains(Domain(TreiberPoolLow, loc_t), One(loc_n)) ==>
+              (var loc_n' := Map_At(Map_At(TreiberPoolLow, One(loc_t))->nodes, One(loc_n))->next;
+                loc_n' is None || Set_Contains(Domain(TreiberPoolLow, loc_t), One(loc_n'->t))));
 
 yield invariant {:layer 2} LocInStackOrNone(loc_t: LocTreiber X, loc_n: Option (LocNode X));
-preserves Map_Contains(TreiberPoolLow, loc_t);
-preserves loc_n is None || Set_Contains(Domain(TreiberPoolLow, loc_t), loc_n->t);
+preserves Map_Contains(TreiberPoolLow, One(loc_t));
+preserves loc_n is None || Set_Contains(Domain(TreiberPoolLow, loc_t), One(loc_n->t));
 
 yield invariant {:layer 3} LocInStack(loc_t: LocTreiber X, loc_n: LocNode X);
-preserves Map_Contains(TreiberPoolLow, loc_t);
-preserves Set_Contains(Domain(TreiberPoolLow, loc_t), loc_n);
+preserves Map_Contains(TreiberPoolLow, One(loc_t));
+preserves Set_Contains(Domain(TreiberPoolLow, loc_t), One(loc_n));
 
 yield invariant {:layer 4} ReachInStack(loc_t: LocTreiber X);
-preserves Map_Contains(TreiberPoolLow, loc_t);
-preserves (var t := TreiberPoolLow->val[loc_t]; Between(t->nodes->val, t->top, t->top, None()));
-preserves (var t := TreiberPoolLow->val[loc_t]; IsSubset(BetweenSet(t->nodes->val, t->top, None()), Domain(TreiberPoolLow, loc_t)->val));
-preserves (var loc_n := Map_At(TreiberPoolLow, loc_t)->top; loc_n is None || Set_Contains(Domain(TreiberPoolLow, loc_t), loc_n->t));
-preserves Map_At(TreiberPool, loc_t) == Abs(Map_At(TreiberPoolLow, loc_t));
+preserves Map_Contains(TreiberPoolLow, One(loc_t));
+preserves (var t := Map_At(TreiberPoolLow, One(loc_t)); Between(t->nodes->val, t->top, t->top, None()));
+preserves (var t := Map_At(TreiberPoolLow, One(loc_t)); ListInDomain(t));
+preserves (var loc_n := Map_At(TreiberPoolLow, One(loc_t))->top; loc_n is None || Set_Contains(Domain(TreiberPoolLow, loc_t), One(loc_n->t)));
+preserves Map_At(TreiberPool, One(loc_t)) == Abs(Map_At(TreiberPoolLow, One(loc_t)));
 
 yield invariant {:layer 4} StackDom();
 preserves TreiberPool->dom == TreiberPoolLow->dom;
 
 yield invariant {:layer 4} PushLocInStack(loc_t: LocTreiber X, node: Node X, new_loc_n: LocNode X, {:linear} tagged_loc: One (TaggedLocNode X));
-preserves Map_Contains(TreiberPoolLow, loc_t);
-preserves Set_Contains(Domain(TreiberPoolLow, loc_t), new_loc_n);
+preserves Map_Contains(TreiberPoolLow, One(loc_t));
+preserves Set_Contains(Domain(TreiberPoolLow, loc_t), One(new_loc_n));
 preserves tagged_loc->val == TaggedLoc(new_loc_n, Unit());
-preserves (var t := TreiberPoolLow->val[loc_t]; Map_At(t->nodes, new_loc_n) == node && !BetweenSet(t->nodes->val, t->top, None())[new_loc_n]);
+preserves (var t := Map_At(TreiberPoolLow, One(loc_t)); Map_At(t->nodes, One(new_loc_n)) == node && !BetweenSet(t->nodes->val, t->top, None())[new_loc_n]);
 
 /// Layered implementation
 
@@ -72,8 +77,8 @@ atomic action {:layer 5} AtomicAlloc() returns ({:linear} tagged_loc: One (Tagge
   call one_loc_t, tagged_locs := TaggedLocSet_New(UnitSet());
   tagged_loc := One(TaggedLoc(one_loc_t->val, Unit()));
   call One_Split(tagged_locs, tagged_loc);
-  assume !Map_Contains(TreiberPool, one_loc_t->val);
-  TreiberPool := Map_Update(TreiberPool, one_loc_t->val, Vec_Empty());
+  assume !Map_Contains(TreiberPool, one_loc_t);
+  TreiberPool := Map_Update(TreiberPool, one_loc_t, Vec_Empty());
 }
 yield procedure {:layer 4} Alloc() returns ({:linear} tagged_loc: One (TaggedLocTreiber X))
 refines AtomicAlloc;
@@ -84,7 +89,7 @@ preserves call StackDom();
   var {:linear} one_loc_t: One (LocTreiber X);
   var {:linear} tagged_locs: Set (TaggedLocTreiber X);
   var top: Option (LocNode X);
-  var {:linear} stack: Map (LocNode X) (Node X);
+  var {:linear} stack: Map (One (LocNode X)) (Node X);
   var {:linear} treiber: Treiber X;
 
   top := None();
@@ -94,20 +99,20 @@ preserves call StackDom();
   tagged_loc := One(TaggedLoc(one_loc_t->val, Unit()));
   call One_Split(tagged_locs, tagged_loc);
   call AllocTreiber#0(one_loc_t, treiber);
-  call {:layer 4} TreiberPool := Copy(Map_Update(TreiberPool, one_loc_t->val, Vec_Empty()));
+  call {:layer 4} TreiberPool := Copy(Map_Update(TreiberPool, one_loc_t, Vec_Empty()));
   call {:layer 4} AbsLemma(treiber);
 }
 
 atomic action {:layer 5} AtomicPush(loc_t: LocTreiber X, x: X) returns (success: bool)
 {
   if (*) {
-    TreiberPool := Map_Update(TreiberPool, loc_t, Vec_Append(Map_At(TreiberPool, loc_t), x));
+    TreiberPool := Map_Update(TreiberPool, One(loc_t), Vec_Append(Map_At(TreiberPool, One(loc_t)), x));
     success := true;
   } else {
     success := false;
   }
 }
-yield procedure {:layer 4} Push(loc_t: LocTreiber X, x: X) returns (success: bool)
+yield procedure {:layer 4} {:vcs_split_on_every_assert} Push(loc_t: LocTreiber X, x: X) returns (success: bool)
 refines AtomicPush;
 preserves call TopInStack(loc_t);
 preserves call ReachInStack(loc_t);
@@ -118,15 +123,15 @@ preserves call StackDom();
   var {:linear} tagged_loc: One (TaggedLocNode X);
   var {:layer 4} old_treiber: Treiber X;
 
-  call {:layer 4} old_treiber := Copy(TreiberPoolLow->val[loc_t]);
+  call {:layer 4} old_treiber := Copy(TreiberPoolLow->val[One(loc_t)]);
   call loc_n, new_loc_n, tagged_loc := CreateNewTopOfStack(loc_t, x);
-  call {:layer 4} FrameLemma(old_treiber, TreiberPoolLow->val[loc_t]);
+  call {:layer 4} FrameLemma(old_treiber, TreiberPoolLow->val[One(loc_t)]);
   call ReachInStack(loc_t) | StackDom() | PushLocInStack(loc_t, Node(loc_n, x), new_loc_n, tagged_loc);
   call success := WriteTopOfStack#0(loc_t, loc_n, Some(new_loc_n));
   if (success) {
-    call {:layer 4} TreiberPool := Copy(Map_Update(TreiberPool, loc_t, Vec_Append(Map_At(TreiberPool, loc_t), x)));
-    assert {:layer 4} TreiberPoolLow->val[loc_t]->top != None();
-    call {:layer 4} AbsLemma(TreiberPoolLow->val[loc_t]);
+    call {:layer 4} TreiberPool := Copy(Map_Update(TreiberPool, One(loc_t), Vec_Append(Map_At(TreiberPool, One(loc_t)), x)));
+    assert {:layer 4} TreiberPoolLow->val[One(loc_t)]->top != None();
+    call {:layer 4} AbsLemma(TreiberPoolLow->val[One(loc_t)]);
   }
 }
 
@@ -135,10 +140,10 @@ atomic action {:layer 5} AtomicPop(loc_t: LocTreiber X) returns (success: bool, 
   var stack: Vec X;
 
   if (*) {
-    stack := Map_At(TreiberPool, loc_t);
+    stack := Map_At(TreiberPool, One(loc_t));
     if (Vec_Len(stack) > 0) {
       x_opt := Some(Vec_Nth(stack, Vec_Len(stack) - 1));
-      TreiberPool := Map_Update(TreiberPool, loc_t, Vec_Remove(stack));
+      TreiberPool := Map_Update(TreiberPool, One(loc_t), Vec_Remove(stack));
     } else {
       x_opt := None();
     }
@@ -154,35 +159,36 @@ preserves call TopInStack(loc_t);
 preserves call ReachInStack(loc_t);
 preserves call StackDom();
 {
-  call {:layer 4} AbsLemma(TreiberPoolLow->val[loc_t]);
+  call {:layer 4} AbsLemma(TreiberPoolLow->val[One(loc_t)]);
   call success, x_opt := PopIntermediate(loc_t);
   if (x_opt is Some) {
-    assert {:layer 4} Vec_Len(Map_At(TreiberPool, loc_t)) > 0;
-    call {:layer 4} TreiberPool := Copy(Map_Update(TreiberPool, loc_t, Vec_Remove(Map_At(TreiberPool, loc_t))));
+    assert {:layer 4} Vec_Len(Map_At(TreiberPool, One(loc_t))) > 0;
+    call {:layer 4} TreiberPool := Copy(Map_Update(TreiberPool, One(loc_t), Vec_Remove(Map_At(TreiberPool, One(loc_t)))));
   }
 }
 
 atomic action {:layer 4} AtomicCreateNewTopOfStack(loc_t: LocTreiber X, x: X)
   returns (loc_n: Option (LocNode X), new_loc_n: LocNode X, {:linear} tagged_loc: One (TaggedLocNode X))
-asserts Map_Contains(TreiberPoolLow, loc_t);
+asserts Map_Contains(TreiberPoolLow, One(loc_t));
 {
   var {:linear} one_loc_t: One (LocTreiber X);
   var {:linear} treiber: Treiber X;
   var top: Option (LocNode X);
-  var {:linear} stack: Map (LocNode X) (Node X);
+  var {:linear} stack: Map (One (LocNode X)) (Node X);
   var {:linear} one_loc_n: One (LocNode X);
   var {:linear} tagged_locs: Set (TaggedLocNode X);
   
-  call one_loc_t, treiber := Map_Get(TreiberPoolLow, loc_t);
+  one_loc_t := One(loc_t);
+  call treiber := Map_GetValue(TreiberPoolLow, one_loc_t);
   Treiber(top, stack) := treiber;
-  assume loc_n is None || Map_Contains(stack, loc_n->t);
+  assume loc_n is None || Map_Contains(stack, One(loc_n->t));
   call one_loc_n, tagged_locs := TaggedLocSet_New(UnitSet());
   new_loc_n := one_loc_n->val;
   tagged_loc := One(TaggedLoc(new_loc_n, Unit()));
   call One_Split(tagged_locs, tagged_loc);
-  call Map_Put(stack, one_loc_n, Node(loc_n, x));
+  call Map_PutValue(stack, one_loc_n, Node(loc_n, x));
   treiber := Treiber(top, stack);
-  call Map_Put(TreiberPoolLow, one_loc_t, treiber);
+  call Map_PutValue(TreiberPoolLow, one_loc_t, treiber);
 }
 yield procedure {:layer 3} CreateNewTopOfStack(loc_t: LocTreiber X, x: X)
   returns (loc_n: Option (LocNode X), new_loc_n: LocNode X, {:linear} tagged_loc: One (TaggedLocNode X))
@@ -207,22 +213,23 @@ atomic action {:layer 4} AtomicPopIntermediate(loc_t: LocTreiber X) returns (suc
   var loc_n: Option (LocNode X);
   var {:linear} treiber: Treiber X;
   var top: Option (LocNode X);
-  var {:linear} stack: Map (LocNode X) (Node X);
+  var {:linear} stack: Map (One (LocNode X)) (Node X);
   var x: X;
 
-  assert Map_Contains(TreiberPoolLow, loc_t);
+  assert Map_Contains(TreiberPoolLow, One(loc_t));
   if (*) {
-    call one_loc_t, treiber := Map_Get(TreiberPoolLow, loc_t);
+    one_loc_t := One(loc_t);
+    call treiber := Map_GetValue(TreiberPoolLow, one_loc_t);
     Treiber(top, stack) := treiber;
-    assume top is Some && Map_Contains(stack, top->t);
-    Node(loc_n, x) := Map_At(stack, top->t);
+    assume top is Some && Map_Contains(stack, One(top->t));
+    Node(loc_n, x) := Map_At(stack, One(top->t));
     treiber := Treiber(loc_n, stack);
-    call Map_Put(TreiberPoolLow, one_loc_t, treiber);
+    call Map_PutValue(TreiberPoolLow, one_loc_t, treiber);
     x_opt := Some(x);
     success := true;
   }
   else if (*) {
-    assume Map_At(TreiberPoolLow, loc_t)->top is None;
+    assume Map_At(TreiberPoolLow, One(loc_t))->top is None;
     x_opt := None();
     success := true;
   } else {
@@ -260,8 +267,8 @@ yield procedure {:layer 2} ReadTopOfStack#Push(loc_t: LocTreiber X) returns (loc
 preserves call TopInStack(loc_t);
 ensures call LocInStackOrNone(loc_t, loc_n);
 refines right action {:layer 3} _ {
-  assert Map_Contains(TreiberPoolLow, loc_t);
-  assume loc_n is None || Set_Contains(Domain(TreiberPoolLow, loc_t), loc_n->t);
+  assert Map_Contains(TreiberPoolLow, One(loc_t));
+  assume loc_n is None || Set_Contains(Domain(TreiberPoolLow, loc_t), One(loc_n->t));
 }
 {
   call loc_n := ReadTopOfStack#0(loc_t);
@@ -272,8 +279,8 @@ preserves call TopInStack(loc_t);
 ensures call LocInStackOrNone(loc_t, loc_n);
 refines atomic action {:layer 3} _
 {
-  assert Map_Contains(TreiberPoolLow, loc_t);
-  assume if loc_n is None then Map_At(TreiberPoolLow, loc_t)->top is None else Set_Contains(Domain(TreiberPoolLow, loc_t), loc_n->t);
+  assert Map_Contains(TreiberPoolLow, One(loc_t));
+  assume if loc_n is None then Map_At(TreiberPoolLow, One(loc_t))->top is None else Set_Contains(Domain(TreiberPoolLow, loc_t), One(loc_n->t));
 }
 {
   call loc_n := ReadTopOfStack#0(loc_t);
@@ -281,9 +288,9 @@ refines atomic action {:layer 3} _
 
 right action {:layer 2,3} AtomicLoadNode#1(loc_t: LocTreiber X, loc_n: LocNode X) returns (node: Node X)
 {
-  assert Map_Contains(TreiberPoolLow, loc_t);
-  assert Map_Contains(Map_At(TreiberPoolLow, loc_t)->nodes, loc_n);
-  node := Map_At(Map_At(TreiberPoolLow, loc_t)->nodes, loc_n);
+  assert Map_Contains(TreiberPoolLow, One(loc_t));
+  assert Map_Contains(Map_At(TreiberPoolLow, One(loc_t))->nodes, One(loc_n));
+  node := Map_At(Map_At(TreiberPoolLow, One(loc_t))->nodes, One(loc_n));
 }
 
 /// Primitives
@@ -294,15 +301,17 @@ refines AtomicLoadNode#1;
   var {:linear} one_loc_t: One (LocTreiber X);
   var {:linear} treiber: Treiber X;
   var top: Option (LocNode X);
-  var {:linear} stack: Map (LocNode X) (Node X);
+  var {:linear} stack: Map (One (LocNode X)) (Node X);
   var {:linear} one_loc_n: One (LocNode X);
 
-  call one_loc_t, treiber := Map_Get(TreiberPoolLow, loc_t);
+  one_loc_t := One(loc_t);
+  call treiber := Map_GetValue(TreiberPoolLow, one_loc_t);
   Treiber(top, stack) := treiber;
-  call one_loc_n, node := Map_Get(stack, loc_n);
-  call Map_Put(stack, one_loc_n, node);
+  one_loc_n := One(loc_n);
+  call node := Map_GetValue(stack, one_loc_n);
+  call Map_PutValue(stack, one_loc_n, node);
   treiber := Treiber(top, stack);
-  call Map_Put(TreiberPoolLow, one_loc_t, treiber);
+  call Map_PutValue(TreiberPoolLow, one_loc_t, treiber);
 }
 yield procedure {:layer 0} LoadNode#0(loc_t: LocTreiber X, loc_n: LocNode X) returns (node: Node X);
 refines AtomicLoadNode#0;
@@ -313,9 +322,10 @@ refines atomic action {:layer 1,2} _
   var {:linear} one_loc_t: One (LocTreiber X);
   var {:linear} treiber: Treiber X;
 
-  call one_loc_t, treiber := Map_Get(TreiberPoolLow, loc_t);
+  one_loc_t := One(loc_t);
+  call treiber := Map_GetValue(TreiberPoolLow, one_loc_t);
   loc_n := treiber->top;
-  call Map_Put(TreiberPoolLow, one_loc_t, treiber);
+  call Map_PutValue(TreiberPoolLow, one_loc_t, treiber);
 }
 
 yield procedure {:layer 0} WriteTopOfStack#0(
@@ -325,14 +335,15 @@ refines atomic action {:layer 1,4} _
   var {:linear} one_loc_t: One (LocTreiber X);
   var {:linear} treiber: Treiber X;
 
-  call one_loc_t, treiber := Map_Get(TreiberPoolLow, loc_t);
+  one_loc_t := One(loc_t);
+  call treiber := Map_GetValue(TreiberPoolLow, one_loc_t);
   if (old_loc_n == treiber->top) {
     treiber->top := new_loc_n;
     success := true;
   } else {
     success := false;
   }
-  call Map_Put(TreiberPoolLow, one_loc_t, treiber);
+  call Map_PutValue(TreiberPoolLow, one_loc_t, treiber);
 }
 
 yield procedure {:layer 0} AllocNode#0(loc_t: LocTreiber X, {:linear_in} one_loc_n: One (LocNode X), node: Node X);
@@ -341,15 +352,16 @@ refines atomic action {:layer 1,3} _
   var {:linear} one_loc_t: One (LocTreiber X);
   var {:linear} treiber: Treiber X;
 
-  call one_loc_t, treiber := Map_Get(TreiberPoolLow, loc_t);
-  call Map_Put(treiber->nodes, one_loc_n, node);
-  call Map_Put(TreiberPoolLow, one_loc_t, treiber);
+  one_loc_t := One(loc_t);
+  call treiber := Map_GetValue(TreiberPoolLow, one_loc_t);
+  call Map_PutValue(treiber->nodes, one_loc_n, node);
+  call Map_PutValue(TreiberPoolLow, one_loc_t, treiber);
 }
 
 yield procedure {:layer 0} AllocTreiber#0({:linear_in} one_loc_t: One (LocTreiber X), {:linear_in} treiber: Treiber X);
 refines atomic action {:layer 1,4} _
 {
-  call Map_Put(TreiberPoolLow, one_loc_t, treiber);
+  call Map_PutValue(TreiberPoolLow, one_loc_t, treiber);
 }
 
 /// Proof of abstraction with a manual encoding of termination
@@ -359,7 +371,7 @@ function Abs(treiber: Treiber X): Vec X;
 function {:inline} AbsDefinition(treiber: Treiber X): Vec X {
 if treiber->top == None() then
   Vec_Empty() else
-  (var n := Map_At(treiber->nodes, treiber->top->t);
+  (var n := Map_At(treiber->nodes, One(treiber->top->t));
     (var treiber' := Treiber(n->next, treiber->nodes); 
       Vec_Append(Abs(treiber'), n->val)))
 }
@@ -370,7 +382,7 @@ requires IsSubset(treiber->nodes->dom->val, treiber'->nodes->dom->val);
 requires MapIte(treiber->nodes->dom->val, treiber->nodes->val, MapConst(Default())) ==
          MapIte(treiber->nodes->dom->val, treiber'->nodes->val, MapConst(Default()));
 requires Between(treiber->nodes->val, treiber->top, treiber->top, None());
-requires IsSubset(BetweenSet(treiber->nodes->val, treiber->top, None()), treiber->nodes->dom->val);
+requires ListInDomain(treiber);
 ensures absStack == AbsDefinition(treiber);
 ensures absStack == AbsDefinition(treiber');
 free ensures absStack == Abs(treiber);
@@ -383,8 +395,8 @@ free ensures absStack == Abs(treiber');
       absStack := Vec_Empty();
   } else {
       loc_n := treiber->top;
-      assert Map_Contains(treiber->nodes, loc_n->t);
-      n := Map_At(treiber->nodes, loc_n->t);
+      assert Map_Contains(treiber->nodes, One(loc_n->t));
+      n := Map_At(treiber->nodes, One(loc_n->t));
       // Use well-founded list reachability to prove that recursion will terminate:
       // treiber@caller->top --> treiber@callee->top --> None()
       assert Between(treiber->nodes->val, loc_n, n->next, None());
@@ -397,7 +409,7 @@ free ensures absStack == Abs(treiber');
 
 pure procedure AbsLemma(treiber: Treiber X)
 requires Between(treiber->nodes->val, treiber->top, treiber->top, None());
-requires IsSubset(BetweenSet(treiber->nodes->val, treiber->top, None()), treiber->nodes->dom->val);
+requires ListInDomain(treiber);
 ensures Abs(treiber) == AbsDefinition(treiber);
 {
   var absStack: Vec X;
@@ -410,7 +422,7 @@ requires IsSubset(treiber->nodes->dom->val, treiber'->nodes->dom->val);
 requires MapIte(treiber->nodes->dom->val, treiber->nodes->val, MapConst(Default())) ==
          MapIte(treiber->nodes->dom->val, treiber'->nodes->val, MapConst(Default()));
 requires Between(treiber->nodes->val, treiber->top, treiber->top, None());
-requires IsSubset(BetweenSet(treiber->nodes->val, treiber->top, None()), treiber->nodes->dom->val);
+requires ListInDomain(treiber);
 ensures Abs(treiber) == Abs(treiber');
 {
   var absStack: Vec X;
